update formalization.lean

RunTime/src/Formalization.lean
@@ -3,31 +3,62 @@ import data.list.sort
 variables {α : Type} (r : α → α → Prop) [decidable_rel r]
 local infix ` ≼ ` : 50 := r
 
-@[simp] def go (b : α) (l : list α × ℕ) : (list α × ℕ) := (b :: l.fst, l.snd + 1)
+namespace counting
+
+@[simp] def go_oi (h : α) (p : list α × ℕ) : (list α × ℕ) := (h :: p.fst, p.snd + 1)
+-- | (l, n) := (b :: l, n + 1)
 
 -- the second value in the output is the number of comparisons made
 @[simp] def ordered_insert (a : α) : list α → (list α × ℕ)
-| [] := ([a], 0)
-| (b :: l) := if a ≼ b then (a :: b :: l, 1)
-                       else go b (ordered_insert l)
-                       -- else let (l', n) := ordered_insert l in (b :: l', n + 1)
+| []       := ([a], 0)
+| (h :: t) := if a ≼ h then (a :: h :: t, 0)
+                       -- else go_oi h (ordered_insert t)
+                       else let (l', n) := ordered_insert t in (h :: l', n + 1)
+
+-- @[simp] def go_is (p₁ : (list α × ℕ)) : (list α × ℕ) :=
 
 @[simp] def insertion_sort : list α → (list α × ℕ)
 | [] := ([], 0)
-| (a :: l) := let (l', n) := (insertion_sort l) , (l'', m) := ordered_insert r a l'
+-- | (h :: t) := go_is (insertion_sort t)
+| (h :: t) := let (l', n) := (insertion_sort t) , (l'', m) := ordered_insert r h l'
               in (l'', n + m)
 
+-- @[simp] def smaller_prefix (a : α) (l : list α) : ℕ := (list.take_while (λ m , m ≼ a) l).length
+@[simp] def smaller_prefix (a : α) : list α → ℕ
+| []       := 0
+| (h :: t) := if a ≼ h then 0 else 1 + smaller_prefix t
 
-theorem ordered_insert_linear (a : α) : ∀ l : list α, (ordered_insert r a l).snd ≤ l.length
+end counting
+
+theorem ordered_insert_linear (a : α) : ∀ l : list α, (counting.ordered_insert r a l).snd ≤ l.length
 | [] := by simp
-| (b :: l) :=
+| (h :: t) :=
 begin
   simp,
   split_ifs,
   { simp, },
-  { have ih : (ordered_insert r a l).snd + 1 ≤ l.length + 1 := nat.pred_le_iff.mp (ordered_insert_linear l),
-    refine le_trans _ ih,
-    refine eq.ge _,
-    exact rfl,
+  {  }
+end
+
+theorem ordered_insert_identification (a : α) : ∀ l : list α,
+  (counting.ordered_insert r a l).fst = list.ordered_insert r a l := sorry
+
+theorem counting_comparisons_oi (a : α) : ∀ l : list α,
+  (counting.ordered_insert r a l).snd = counting.smaller_prefix (≼) a l
+| []       := by simp
+| (h :: t) :=
+begin
+  simp,
+  split_ifs,
+  { simp },
+  { rw counting_comparisons_oi t,
+    exact add_comm (counting.smaller_prefix r a t) 1
   }
 end
+
+theorem insertion_sort_quadratic : ∀ l : list α, (counting.insertion_sort r l).snd ≤ l.length * l.length
+| []       := by simp
+| (h :: t) := sorry
+
+theorem insertion_sort_identification (a : α) : ∀ l : list α,
+  (counting.insertion_sort r l).fst = list.insertion_sort r l := sorry
